examples/Monad2/MonadExpr.v
@@ -28,7 +28,7 @@ Section mext.
   Definition exprD (ts : list Type) (us vs : EnvI.env typD) (t : typ) (e : mexpr) : option (typD ts t) :=
     let (tus,us) := EnvI.split_env us in
     let (tvs,vs) := EnvI.split_env vs in
-    match @ExprDenote.exprD' typ typD mext
+    match @exprD' typ typD mext
                              (RType_typ _ _) _ RSym_mext
                              ts tus tvs t e
     with
