theories/Lambda/ExprCore.v
@@ -1,5 +1,7 @@
 Require Import Coq.Bool.Bool.
 Require Import ExtLib.Core.RelDec.
+Require Import ExtLib.Relations.TransitiveClosure.
+Require Import ExtLib.Recur.Relation.
 Require Import ExtLib.Tactics.Consider.
 Require Import MirrorCore.EnvI.
 Require Import MirrorCore.ExprI.
@@ -38,6 +40,21 @@ Section env.
     { inversion H; clear H; subst; auto. }
   Qed.
 
+
+  Theorem expr_strong_ind
+  : forall (P : expr -> Prop),
+      (forall v, P (Var v)) ->
+      (forall u, P (UVar u)) ->
+      (forall i, P (Inj i)) ->
+      (forall a b, (forall e, (leftTrans expr_acc) e (App a b) -> P e) -> P (App a b)) ->
+      (forall t a, (forall e, (leftTrans expr_acc) e (Abs t a) -> P e) -> P (Abs t a)) ->
+      forall e, P e.
+  Proof.
+    intros P Hvar Huvar Hinj Happ Habs.
+    eapply Fix. eapply wf_leftTrans. eapply wf_expr_acc.
+    destruct x; auto.
+  Qed.
+
   Variable RelDec_eq_typ : RelDec (@eq typ).
   Variable RelDec_eq_func : RelDec (@eq func).
 
@@ -66,7 +83,6 @@ Section env.
   Theorem expr_eq_dec_eq : forall e1 e2,
     expr_eq_dec e1 e2 = true <-> e1 = e2.
   Proof.
-(*
     induction e1; destruct e2; simpl; intros;
     repeat match goal with
              | |- context [ if ?X then ?Y else false ] =>
@@ -76,9 +92,6 @@ Section env.
                  rewrite rel_dec_correct
              | |- context [ ?X ?[ ?Z ] ?Y ] =>
                rewrite rel_dec_correct
-             | |- context [ type_eqb ?X ?Y ] =>
-               change (type_eqb X Y) with (X ?[ eq ] Y) ;
-                 rewrite rel_dec_correct
              | |- context [ ?X ?[ @eq ?T ]?Y ] =>
                change (X ?[ @eq T ] Y) with (X ?[ eq ] Y) ;
                  rewrite rel_dec_correct
@@ -88,8 +101,7 @@ Section env.
              | |- _ => rewrite andb_true_iff
              | H : forall x, (_ = true) <-> _ |- _ => rewrite H
            end; try solve [ intuition congruence ].
-*)
-  Admitted.
+  Qed.
 
   Global Instance RelDec_eq_expr : RelDec (@eq expr) :=
   { rel_dec := expr_eq_dec }.
